
\section*{Ex 1.3}
\begin{mdframed}
	\textbf{Prove:} \\
	let $L_1 \subseteq \Sigma^*$
	\[
		\left( \forall x,y \in L_1 :\: xy = yx \right) \implies \left( \exists \omega \in \Sigma^* :\: L_1 \subseteq \{\omega\}^* \right)
	\]
\end{mdframed}

\begin{proof}
First we need to proof that $(\forall x,y \in L_1 \; xy=yx) \implies 
(\exists \omega \in \Sigma,\; p,q >0:\; x = \omega^p, y = \omega^q)$.
The proof will be by induction on $|xy|$.\\

\hfill\begin{minipage}{\dimexpr\textwidth-1cm}
\begin{proof}
	\subsection*{Base case}
	Let $|xy| = 2$. (If $|xy|=1$ then $x=\varepsilon$ or $y=\varepsilon$. Obviously $xy=yx$)
	Then $|x| = |y| = 1$ and obviously $x = y$. That is, $\omega = x = y$, $p=q=1$

	\subsection*{Induction}
	Let implication true $\forall x,y :\; |xy| < n$. We prove it for $|xy| = n$.
	Without loss of generality we can sat that $|x| >= |y|$. If not so, just swap them.
	\begin{align*}
		& \begin{pmatrix}
		x_1 & x_2 & x_3 & x_4 & x_5 & ... & x_{|x|} & y_1 & ... & y_{|y|} \\
		y_1 & ... & y_{|y|} & x_1 & x_2 & x_3 & x_4 & x_5 & ... & x_{|x|} 
		\end{pmatrix}; \\
		& (xy)_i = (yx)_i \\
		& \implies \exists z \in \Sigma^* :\; x = zy = yz
	\end{align*}
	If $|z| = 0$, $x=y$ and we can take $\omega = x, p=q=1$.
	Otherwise, $z \in \Sigma^+$ and $|zy| < n$. 
	Induction hypothesis applies: $\exists \omega \in \Sigma,\; p',q' >0:\; z = \omega^{p'}, y = \omega^{q'}$.\\
	Then, $x = zy = \omega^{p'} \omega^{q'} = \omega^{p' + q'}$ and $y = \omega^{q'}$
\end{proof}
\end{minipage}
\\ \\
So we know that $\forall x,y \in L_1 \; \exists \omega \in \Sigma,\; p,q \ge 0:\; x = \omega^p, y = \omega^q$.
In other words, $x,y \in \{\omega\}^*$ and even $x \in \{\omega\}^*$.
That is, $L_1 \subseteq \{\omega\}^*$
\end{proof}
