\section*{Ex 1.5}
\begin{mdframed}
	\textbf{Prove:} \\
	let $\varepsilon \notin \Sigma$
	\[
		\forall L_1 \subseteq \Sigma^* :\: (L_1^* = L_1 L_1^*) \iff (\varepsilon \in L_1)
	\]
\end{mdframed}

% \begin{proof}

% 	1. $\implies$

% 	We got $L_1^* = L_1 L_1^*$. % Let $\varepsilon \notin L_1$.
% 	Note that $\varepsilon \in L_1^*$ by definition. 
% 	Then $\varepsilon \in L_1 L_1^*$. \\
% 	So $\varepsilon \in L_1 \left(\{\varepsilon\} \cup \bigcup_{n=1}^\infty L_1^n\right)$.\\
% 	$\varepsilon \in \{x_0 x_1 x_2 \dots x_n \;|\; x_0 \in L_1,\; x_i \in (L_1\cup\{\varepsilon\}),\; n>0\}$.\\
% 	Even if $x_i = \varepsilon, i>0$ we have $\varepsilon \in \{x_0 | x_0 \in L_1\} \in $ left.
% 	$\varepsilon \in L_1$.
% \end{proof}

\begin{proof}

	% 2. $\impliedby$

	% We got $\varepsilon \in L_1$. 
	
	% Let $x \in L_1^*$. Words from RHS have a form of $a b \;|\; a\in L_1, b\in L_1^*$.
	% Let $a = \varepsilon, b = x \implies \varepsilon x \in$ RHS. 
	% That is, $L_1^* \subseteq L_1 L_1^*$.

	% Let $x \in L_1 L_1^*$. 
	\begin{align*}
		L_1 L_1^* & = L_1 \left(\{\varepsilon\} \cup \bigcup_{n=1}^\infty L_1^n\right) = 
		L_1 \cup  \bigcup_{n=2}^\infty L_1^n = \\ & = \bigcup_{n=1}^\infty L_1^n; \\
		L_1^* & = \left(\bigcup_{n=1}^\infty L_1^n\right) \cup \{\varepsilon\};
	\end{align*}

	Obviously, $L_1 L_1^* \subseteq L_1^*$. Question is wether $L_1^* \subseteq L_1 L_1^*$. \\

	1. $\implies$ \\
	Let $x \in L_1^* \implies x \in L_1 L_1^*$. 
	Let $x = \varepsilon \in L_1^*$. Then $\varepsilon \in \bigcup_{n=1}^\infty L_1^n$.
	This could be true only when $\varepsilon \in L_1$. \qedsymbol 

	2. $\impliedby$ \\
	Let $\varepsilon \in L_1$.
	Then $L_1 = L_1 \cup \{\varepsilon\}$. 
	Let $x \in L_1^*$. If $x \ne \varepsilon$, obviously $x \in L_1 L_1^*$.
	If $x = \varepsilon$ we got
	\begin{align*}
		L_1 L_1^* & = \bigcup_{n=1}^\infty L_1^n = \bigcup_{n=1}^\infty (L_1 \cup \{\varepsilon\})^n = \\
		& = L_1 \cup \{\varepsilon\} \cup \bigcup_{n=2}^\infty L_1^n
	\end{align*}
	So, $x \in L_1 L_1^*$. \qedsymbol

	That is, $(L_1^* = L_1 L_1^*) \iff (\varepsilon \in L_1)$
\end{proof}